theories/ast.v
@@ -1,0 +1,155 @@
+From Ssreflect
+Require Import ssreflect ssrfun ssrbool ssrnat eqtype choice seq fintype.
+From MathComp
+Require Import bigop  finfun finset generic_quotient perm tuple fingroup.
+From Nominal
+Require Import finmap finsfun finperm nominal.
+
+Set Implicit Arguments.
+Unset Strict Implicit.
+Unset Printing Implicit Defensive.
+
+Delimit Scope finperm_scope with fperm.
+Local Open Scope finperm_scope.
+Local Open Scope fset.
+Local Open Scope quotient_scope.
+
+Import Key.Exports.
+
+Section ASTDef.
+
+Variables (node_label : Type) (leaf_type: nominalType atom).
+
+Inductive rAST := 
+|rLeaf of leaf_type
+|rCons of node_label & seq rAST
+|rBinderCons of node_label * atom & seq rAST.
+
+
+(* TODO : encodage des rAST *)
+Definition rAST_encode : rAST -> GenTree.tree atom. Admitted.
+Definition rAST_decode : GenTree.tree atom -> rAST. Admitted.
+Lemma rAST_codeK : cancel rAST_encode rAST_decode. Admitted.
+
+Definition rAST_eqMixin := CanEqMixin rAST_codeK.
+Canonical rAST_eqType := EqType rAST rAST_eqMixin.
+Definition rAST_choiceMixin := CanChoiceMixin rAST_codeK.
+Canonical rAST_choiceType := ChoiceType rAST rAST_choiceMixin.
+Definition rAST_countMixin := CanCountMixin rAST_codeK.
+Canonical rAST_countType := CountType rAST rAST_countMixin.
+
+Definition rAST_better_rect T IH_leaf IH_cons IH_bcons :=
+  fix loop t : T  := 
+  let fix result_list f : seq T :=
+      if f is t :: f' then loop t :: (result_list f') else nil
+  in
+  match t with
+  | rLeaf x => IH_leaf x
+  | rCons c f0 => IH_cons c f0 (result_list f0)
+  | rBinderCons (c, x) f0 => IH_bcons (c,x) f0 (result_list f0) 
+    end.
+
+Lemma rAST_better_ind_subproof (P : rAST -> Prop) (f : seq rAST): 
+ foldr (fun t => and (P t)) True f -> (forall t, t \in f -> P t).
+Proof.
+elim: f => [|t l IHl] //=. 
+move => [Ptt P_all_l] u. 
+rewrite inE => /orP. case; first by move /eqP ->.
+by apply IHl.
+Qed.
+
+Definition rAST_better_ind P IH_leaf IH_cons IH_bcons :=
+  fix loop t : P t : Prop := 
+  let fix iter_conj f : foldr (fun t => and (P t)) True f :=
+      if f is t :: f' then conj (loop t) (iter_conj f') else Logic.I
+  in
+  match t with
+  | rLeaf x => IH_leaf x
+  | rCons c f0 => IH_cons c f0 (rAST_better_ind_subproof (iter_conj f0))
+  | rBinderCons (c, x) f0 => IH_bcons (c,x) f0 (rAST_better_ind_subproof (iter_conj f0))
+    end.
+
+Definition rAST_depth : rAST -> nat.
+apply/rAST_better_rect => [_|_ _ l|_ _ l].
+  - exact: 0. 
+  - exact: (foldr maxn 0 l).+1.
+  - exact: (foldr maxn 0 l).+1.
+Defined.
+
+Fixpoint rAST_act (π : {finperm atom}) (t : rAST) :=
+  match t with
+    |rLeaf u => rLeaf (π \dot u)
+    |rCons c l => rCons c [seq (rAST_act π u) | u <- l]
+    |rBinderCons (c, x) l => rBinderCons (c, π x) [seq (rAST_act π u) | u <- l]
+  end.
+
+Lemma rAST_act1 : rAST_act (1 atom) =1 id.
+Proof. 
+elim/rAST_better_ind => [x|c l IHl|[c x] l IHl] /=.
+  - by rewrite act1.
+  - by rewrite map_id_in //.
+  - by rewrite finsfun1 map_id_in.
+Qed.
+
+Lemma rAST_actM π π' (t : rAST) : 
+  rAST_act (π * π') t = rAST_act π (rAST_act π' t).
+Proof.
+elim/rAST_better_ind :t => [x|c l IHl|[c x] l IHl] /=.
+  - by rewrite actM.
+  - congr rCons. rewrite -map_comp. 
+    apply eq_in_map => t /=. exact: IHl.
+  - congr rBinderCons. 
+      by rewrite finsfunM.
+    rewrite -map_comp. apply eq_in_map => t /=.
+    exact: IHl.
+Qed.
+
+Lemma rAST_actproper : forall t1 t2 π, t1 = t2 -> (rAST_act π t1) = (rAST_act π t2).
+Proof. by move => t1 t2 π ->. Qed.
+
+Definition rAST_nominal_setoid_mixin := 
+  @PermSetoidMixin rAST (@eq rAST) atom rAST_act rAST_act1 
+                   rAST_actM rAST_actproper.   
+
+Definition rAST_support : rAST -> {fset atom}.
+apply/rAST_better_rect => [leaf|_ _ children_supports|[_ x] _ children_supports].
+  - exact: support leaf.
+  - exact: (fsetU_list children_supports).
+  - exact: (x |` (fsetU_list children_supports)).
+Defined.
+
+Lemma rAST_cons_support (l : seq rAST) (t : rAST) c :
+  t \in l -> rAST_support t `<=` rAST_support (rCons c l).
+Proof.
+move => t_l. 
+apply/fsubsetP => x x_supp_t.
+apply/fsetU_listP. exists (rAST_support t) => //.
+exact: map_f.
+Qed.
+
+Lemma rAST_act_id (π : {finperm atom}) (t : rAST) :
+     (forall a : atom, a \in rAST_support t -> π a = a) -> rAST_act π t = t.
+Proof.
+elim/rAST_better_ind : t => [x|c l IHl|[c x] l IHl] Hsupp /=.
+  - by rewrite act_id.
+  - rewrite map_id_in // => t t_in_l.
+    apply IHl => // a a_supp_t.
+    exact/Hsupp/(fsubsetP (rAST_cons_support c t_in_l) a). 
+  - rewrite map_id_in.
+      by rewrite Hsupp // fset1U1. 
+    move => t t_in_l.
+    apply IHl => // a a_supp_t.
+    exact/Hsupp/fset1Ur/(fsubsetP (rAST_cons_support c t_in_l) a).
+Qed.
+
+End ASTDef.
+
+Definition rAST_nominal_mixin (node_label : Type) (leaf_type : nominalType atom) :=
+  @NominalMixin (rAST_choiceType node_label leaf_type) atom 
+                (rAST_nominal_setoid_mixin node_label leaf_type) _ 
+                (@rAST_act_id node_label leaf_type).
+
+Canonical rAST_nominalType (node_label : Type) (leaf_type : nominalType atom) := 
+  @NominalType atom
+    (@rAST_choiceType node_label leaf_type) 
+    (@rAST_nominal_mixin node_label leaf_type).
